BAs done.

Semantics.v
@@ -1,74 +1,11 @@
 Set Implicit Arguments.
 
+Require Import Relation.
 Require Import Syntax.
 Require Import Coq.Classes.Equivalence.
 Require Import Coq.Arith.EqNat.
 Require Import Coq.Logic.FunctionalExtensionality.
 Require Import Coq.Setoids.Setoid.
-
-Module Relation.
-
-  Section Defs.
-
-    Variable A : Type.
-    
-    Definition relation := A -> A -> Prop.
-    
-    Definition union (R1 R2 : relation) : relation :=
-      fun (x y : A) => R1 x y \/ R2 x y.
-    
-    Definition join (R1 R2 : relation) : relation :=
-      fun (x y : A) => exists (z : A), R1 x z /\ R2 z y.
-    
-    Definition empty : relation :=
-      fun (x y : A) => False.
-    
-    Definition id : relation :=
-      fun (x y : A) => x = y.
-    
-    Fixpoint expt (R : relation) (n : nat) : relation :=
-      match n with
-        | 0 => id
-        | S m => join R (expt R m)
-      end.
-    
-    Definition star (R : relation) : relation :=
-      fun (x y : A) => exists n, (expt R n) x y.
-
-    Definition equiv (R1 R2 : relation) :=
-      forall (x y : A), R1 x y <-> R2 x y.
-
-   Definition inv (R : relation) : relation :=
-     fun (x y : A) => ((R x y) /\ False) \/ (~(R x y) /\ (x = y)).
-  
-  Definition contains (R1 R2 : relation) : Prop :=
-     forall (x y : A), R1 x y -> R2 x y.
-
-  End Defs.
-
-  Instance Equivalence_equiv `(A : Type) : Equivalence (@equiv A).
-  Proof with auto.
-    split; unfold equiv.
-    + unfold Reflexive.
-      intros. intuition.
-    + unfold Symmetric.
-      intros. symmetry. apply H.
-    + unfold Transitive.
-      intros.
-      split... 
-      - intros.
-        apply H0.
-        apply H...
-      - intros.
-        apply H.
-        apply H0...
-  Qed.
-
-End Relation.
-
-Module Semantics.
-
-  Import Relation.
 
   Definition get_Field (pkt : packet) (fld : field) : nat :=
     match fld with
@@ -94,9 +31,6 @@ Module Semantics.
       | ConsHist p h => p
     end.
 
-  Locate exp.
-  Check exp.
-  Check relation.
   Fixpoint eval (e : exp) : relation history :=
     match e with
       | Drop => @empty history
@@ -115,7 +49,7 @@ Module Semantics.
       | Seq e1 e2 => join (eval e1) (eval e2)
       | Star e1 => star (eval e1)
     end.
-
+(*
   Definition equiv_exp (e1 : exp) (e2 : exp) : Prop := 
     equiv (eval e1) (eval e2).
 
@@ -132,168 +66,5 @@ Module Semantics.
     + unfold Transitive.
       intros.
       eapply transitivity; eauto.
-  Qed.
+  Qed.*)
 
-End Semantics.
-
-Module BooleanAlgebra.
-
-  Import Semantics.
-  Import Syntax.
-  Import Relation.
-
-  Existing Instances Equivalence_exp.
-  Local Open Scope equiv_scope.
-
-
-  (* Predicates are either identity or empty *)
-  Lemma bool_spec : forall (e : exp),
-    pred e ->
-    forall (h r : history),
-      eval e h r -> (False \/ h = r).
-  Proof with auto.
-    intros.
-    generalize dependent h.
-    generalize dependent r.
-    induction H; intros...
-    + unfold eval in H0. 
-    destruct (beq_nat (get_Field (get_Packet h) f) v) in H0...
-    + simpl in H1. unfold union in H1. destruct H1...
-    + simpl in H1. unfold join in H1. destruct H1. destruct H1.
-      apply IHpred1 in H1. destruct H1. contradiction. subst.
-      apply IHpred2 in H2...
-    + simpl in H0. unfold inv in H0. destruct H0. destruct H0. contradiction.
-      unfold not in H0. destruct H0. right...
-  Qed.
-
-  Lemma bool_spec_new : forall (e : exp), pred e -> 
-    contains (eval e) (@id history).
-  Proof with auto.
-    intros. unfold contains.
-    induction H; intros...
-    + simpl in H. unfold empty in H. contradiction.
-    + simpl in H. destruct (beq_nat (get_Field (get_Packet x) f) v) in H...
-      contradiction.
-    + simpl in H1. unfold union in H1. destruct H1...
-    + simpl in H1. unfold join in H1.  destruct H1... destruct H1...
-      apply IHpred1 in H1. apply IHpred2 in H2. unfold id in *. subst...
-    + simpl in H0. unfold inv in H0. destruct H0. destruct H0. contradiction. 
-      unfold not in H0. unfold id. destruct H0...
- Qed. 
-
-  Lemma bool_true_spec : forall (e : exp) (h1 h2 : history),
-    pred e ->
-    eval e h1 h2 ->
-    h1 = h2.
-  Proof with eauto.
-    intros.
-    eapply bool_spec in H...
-    destruct H...
-    contradiction.
-  Qed.
-  
-  Lemma BA_Plus_One : 
-    forall (e : exp),
-      pred e ->
-      (Par e Id) === Id.
-  Proof with auto.
-    intros.
-    split.
-    + intros. simpl in *. 
-      unfold union in H0.
-      destruct H0... apply bool_spec_new in H0...
-    + intros. simpl in *.
-      unfold union...
-   Qed.
-  
-  Lemma BA_Seq_Comm :
-    forall (e1 e2 : exp),
-      pred e1 -> pred e2 ->
-        (Seq e1 e2) === (Seq e2 e1).
-  Proof with eauto. 
-    intros. split. simpl in *.
-    +  intros. unfold join in *. destruct H1...
-       destruct H1.
-       assert (x = x0). eapply bool_true_spec. exact H. trivial.
-       subst.
-       assert (x0 = y). eapply bool_true_spec. exact H0. trivial.
-       subst.
-       exists y...
-     + simpl. unfold join. intros.
-       destruct H1 as [z [H1 H2]].
-       remember H1. clear Heqe.
-       remember H2. clear Heqe0.
-       apply bool_true_spec in H1...
-       apply bool_true_spec in H2...
-       subst...
-    Qed.       
-
-  Lemma BA_Plus_Dist :
-    forall (e1 e2 e3 : exp),
-       pred e1 /\ pred e2 /\ pred e3 ->
-         (Par e1 (Seq e2 e3)) === (Seq (Par e1 e2) (Par e1 e3)).
-  Proof with auto.
-    intros. split.
-    + intros. simpl in *. unfold join in *. unfold union in *.
-      destruct H0.
-      assert (x = y). eapply bool_true_spec. destruct H. exact H. trivial.
-      subst. exists y. split...
-      destruct H0. destruct H0. destruct H. destruct H2. remember H0 as H0'.
-      clear HeqH0'. remember H1 as H1'. clear HeqH1'.
-      eapply bool_true_spec in H0. subst. eapply bool_true_spec in H1. subst.
-      exists y. split... trivial. trivial.
-    + intros.  simpl in *. unfold join in *. unfold union in *.
-      destruct H0. destruct H0. destruct H0. remember H0 as H0'. clear HeqH0'.
-      destruct H. eapply bool_true_spec in H0. subst. destruct H1. left. trivial.
-      destruct H2. eapply bool_true_spec in H0.  subst. left. trivial.
-      trivial. trivial.
-      destruct H1. destruct H. remember H1 as H1'. clear HeqH1'.
-      eapply bool_true_spec in H1. subst. destruct H2. eapply bool_true_spec in H0.
-      subst. left. auto. auto. auto.
-      right. remember H0 as H0'. clear HeqH0'. remember H1 as H1'. clear HeqH1'.
-      destruct H. destruct H2.
-      eapply bool_true_spec in H1. subst. eapply bool_true_spec in H0. subst.
-      exists y. split... trivial. trivial.
-  Qed.
-
-  Lemma BA_Seq_Idem :
-    forall (e : exp),
-      pred e -> (Seq e e) === e.
-  Proof with auto.
-    intros. split.
-    + intros. simpl in *. unfold join in H0. destruct H0...
-      destruct H0... remember H1 as H1'. remember H0 as H0'.
-      clear HeqH0'. clear HeqH1'. apply bool_true_spec in H0...
-      apply bool_true_spec in H1. subst. trivial. trivial.
-    + intros. simpl. unfold join. remember H0 as H0'. clear HeqH0'.
-      apply bool_true_spec in H0... subst. exists y...
-  Qed.
-      
-  Lemma BA_Excl_Mid : 
-    forall (e : exp), 
-      pred e -> (Par e (Neg e)) === Id.
-  Proof with auto.
-    intros.
-    split.
-    + intros. simpl in *.
-      unfold union in H0.
-      unfold inv in H0. unfold id.
-      destruct H0. Focus 2. destruct H0. destruct H0. contradiction.
-      destruct H0... apply bool_spec_new in H0...
-    + intros. assert (x = y). apply bool_true_spec in H0...
-      subst. simpl. unfold union. simpl in H0. unfold id in H0. unfold inv.
-   Admitted.
-
-  Lemma BA_Contra :
-    forall (e : exp),
-      pred e ->
-      (Seq e (Neg e)) === Drop.
-  Proof with auto.
-    intros. split. 
-    + intros. simpl in *. unfold join in H0.
-      destruct H0.  destruct H0. remember H0 as H0'.
-      clear HeqH0'. apply bool_true_spec in H0. subst. unfold inv in H1.
-      destruct H1. destruct H0. contradiction. destruct H0. subst. contradiction.
-      trivial.
-    + intros. simpl in *. unfold empty in H0. contradiction.
-  Qed.        
