BooleanAlgebraAxioms.v
@@ -1,52 +1,206 @@
 Set Implicit Arguments.
 
+Require Import Relation.
 Require Import Syntax.
 Require Import Semantics.
-Require Import Coq.Arith.EqNat.
 Require Import Coq.Classes.Equivalence.
-Require Import Coq.Classes.RelationClasses.
+Require Import Coq.Arith.EqNat.
+Require Import Coq.Logic.FunctionalExtensionality.
 Require Import Coq.Setoids.Setoid.
-Require Import Coq.Sets.Ensembles.
-Require Import Coq.Sets.Constructive_sets.
-Open Local Scope equiv_scope.
-Hint Resolve reflexivity.
 
-Lemma union_set_subset_is_set :
-  forall (A : Type) (seta setb: Ensemble A), @Included _ seta setb -> @Union _  seta setb  = seta.
-Proof with auto. 
-  intros. unfold Included in *. 
-  Print Union.
-  apply Union_introl. 
-Lemma pred_null_or_single :
-  forall (pred1 : exp) (h : history), (pred pred1) -> 
-         (eval pred1 h) = @Empty_set history \/ (eval pred1 h) = (Singleton _ h).
-Proof with auto. intros. 
-  induction pred1; simpl; auto. 
-  destruct beq_nat...
-  inversion H. subst. 
-  apply IHpred1_1 in H2. apply IHpred1_2 in H3.
-  destruct H2; destruct H3. rewrite H0. rewrite H1. auto. left. rewrite -> H0.
-  rewrite -> H1. simpl.
-  apply Union_inv.    
-left. simpl. reflexivity.
+  Existing Instances Equivalence_exp.
+  Local Open Scope equiv_scope.
 
-Lemma ba_plus_one : 
-  forall (pred1 : exp), (pred pred1) -> equiv_exp (Par pred1 (Id)) (Id).
-Proof. intros. unfold equiv_exp. intros. simpl.
 
-Lemma ba_plus_dist : 
-  forall (pred1 pred2 pred3 : pred), (PrPar pred1 (PrSeq pred2 pred3)) 
-          === (PrSeq (PrPar pred1 pred2) (PrPar pred1 pred3)).
+  (* Predicates are either identity or empty *)
+  Lemma bool_spec : forall (e : exp),
+    pred e ->
+    forall (h r : history),
+      eval e h r -> (False \/ h = r).
+  Proof with auto.
+    intros.
+    generalize dependent h.
+    generalize dependent r.
+    induction H; intros...
+    + unfold eval in H0. 
+    destruct (beq_nat (get_Field (get_Packet h) f) v) in H0...
+    + simpl in H1. unfold union in H1. destruct H1...
+    + simpl in H1. unfold join in H1. destruct H1. destruct H1.
+      apply IHpred1 in H1. destruct H1. contradiction. subst.
+      apply IHpred2 in H2...
+    + simpl in H0. unfold inv in H0. destruct H0. destruct H0. contradiction.
+      unfold not in H0. destruct H0. right...
+  Qed.
 
-Lemma ba_excl_mid :
-  forall (pred1 : pred), (PrPar pred1 (PrNeg pred1)) === PrDrop pred1.
+  Lemma bool_spec_new : forall (e : exp), pred e -> 
+    contains (eval e) (@id history).
+  Proof with auto.
+    intros. unfold contains.
+    induction H; intros...
+    + simpl in H. unfold empty in H. contradiction.
+    + simpl in H. destruct (beq_nat (get_Field (get_Packet x) f) v) in H...
+      contradiction.
+    + simpl in H1. unfold union in H1. destruct H1...
+    + simpl in H1. unfold join in H1.  destruct H1... destruct H1...
+      apply IHpred1 in H1. apply IHpred2 in H2. unfold id in *. subst...
+    + simpl in H0. unfold inv in H0. destruct H0. destruct H0. contradiction. 
+      unfold not in H0. unfold id. destruct H0...
+ Qed. 
 
-Lemma ba_seq_comm :
-  forall (pred1 pred2 : pred), (PrSeq pred1 pred2) === (PrSeq pred2 pred1).
+  Lemma bool_true_spec : forall (e : exp) (h1 h2 : history),
+    pred e ->
+    eval e h1 h2 ->
+    h1 = h2.
+  Proof with eauto.
+    intros.
+    eapply bool_spec in H...
+    destruct H...
+    contradiction.
+  Qed.
+  
+  Lemma BA_Plus_One : 
+    forall (e : exp),
+      pred e ->
+      (Par e Id) === Id.
+  Proof with auto.
+    intros.
+    split.
+    + intros. simpl in *. 
+      unfold union in H0.
+      destruct H0... apply bool_spec_new in H0...
+    + intros. simpl in *.
+      unfold union...
+   Qed.
+  
+  Lemma BA_Seq_Comm :
+    forall (e1 e2 : exp),
+      pred e1 -> pred e2 ->
+        (Seq e1 e2) === (Seq e2 e1).
+  Proof with eauto. 
+    intros. split. simpl in *.
+    +  intros. unfold join in *. destruct H1...
+       destruct H1.
+       assert (x = x0). eapply bool_true_spec. exact H. trivial.
+       subst.
+       assert (x0 = y). eapply bool_true_spec. exact H0. trivial.
+       subst.
+       exists y...
+     + simpl. unfold join. intros.
+       destruct H1 as [z [H1 H2]].
+       remember H1. clear Heqe.
+       remember H2. clear Heqe0.
+       apply bool_true_spec in H1...
+       apply bool_true_spec in H2...
+       subst...
+    Qed.       
 
-Lemma ba_contra :
-  forall (pred1 : pred), (PrSeq pred1 (PrNeg pred1)) === PrDrop pred1.
+  Lemma BA_Plus_Dist :
+    forall (e1 e2 e3 : exp),
+       pred e1 /\ pred e2 /\ pred e3 ->
+         (Par e1 (Seq e2 e3)) === (Seq (Par e1 e2) (Par e1 e3)).
+  Proof with auto.
+    intros. split.
+    + intros. simpl in *. unfold join in *. unfold union in *.
+      destruct H0.
+      assert (x = y). eapply bool_true_spec. destruct H. exact H. trivial.
+      subst. exists y. split...
+      destruct H0. destruct H0. destruct H. destruct H2. remember H0 as H0'.
+      clear HeqH0'. remember H1 as H1'. clear HeqH1'.
+      eapply bool_true_spec in H0. subst. eapply bool_true_spec in H1. subst.
+      exists y. split... trivial. trivial.
+    + intros.  simpl in *. unfold join in *. unfold union in *.
+      destruct H0. destruct H0. destruct H0. remember H0 as H0'. clear HeqH0'.
+      destruct H. eapply bool_true_spec in H0. subst. destruct H1. left. trivial.
+      destruct H2. eapply bool_true_spec in H0.  subst. left. trivial.
+      trivial. trivial.
+      destruct H1. destruct H. remember H1 as H1'. clear HeqH1'.
+      eapply bool_true_spec in H1. subst. destruct H2. eapply bool_true_spec in H0.
+      subst. left. auto. auto. auto.
+      right. remember H0 as H0'. clear HeqH0'. remember H1 as H1'. clear HeqH1'.
+      destruct H. destruct H2.
+      eapply bool_true_spec in H1. subst. eapply bool_true_spec in H0. subst.
+      exists y. split... trivial. trivial.
+  Qed.
 
-Lemma ba_seq_idem :
-  forall (pred1 : pred), (PrSeq pred1 pred1) === pred1.
+  Lemma BA_Seq_Idem :
+    forall (e : exp),
+      pred e -> (Seq e e) === e.
+  Proof with auto.
+    intros. split.
+    + intros. simpl in *. unfold join in H0. destruct H0...
+      destruct H0... remember H1 as H1'. remember H0 as H0'.
+      clear HeqH0'. clear HeqH1'. apply bool_true_spec in H0...
+      apply bool_true_spec in H1. subst. trivial. trivial.
+    + intros. simpl. unfold join. remember H0 as H0'. clear HeqH0'.
+      apply bool_true_spec in H0... subst. exists y...
+  Qed.
+      
+  Lemma either_or : 
+    forall (e : exp) (x : history),
+      pred e -> (eval e x x) \/ ~(eval e x x).
+  Proof with auto.
+    intros.
+    induction e.
+    + intuition.
+    + intuition.
+    + simpl. destruct (beq_nat (get_Field (get_Packet x) f) n). left. reflexivity.
+      unfold not. right. intros. trivial.
+    + simpl in *. unfold union. destruct IHe1. inversion H. trivial. destruct IHe2.
+      inversion H. trivial. left. intuition. left. intuition. inversion H. 
+      apply IHe2 in H4. destruct H4. left. right. trivial. right. unfold not in *.
+      intuition.
+    + inversion H. apply IHe1 in H2. apply IHe2 in H3. clear IHe1 IHe2. 
+      subst. simpl in *. unfold join.
+       destruct H2; destruct H3. 
+       - left. exists x. intuition.
+       - right. unfold not. intros. destruct H2 as [z [H2 H3]].
+         remember H3 as H3'. clear HeqH3'. apply bool_true_spec in H3. subst. contradiction.
+         inversion H. trivial.
+       - right. unfold not. intros. destruct H2 as [z [H2 H3]].
+         remember H2 as H2'. clear HeqH2'. apply bool_true_spec in H2. subst. contradiction.
+         inversion H. trivial.
+       - right. unfold not. intros. destruct H2. destruct H2. remember H2 as H2'.
+         clear HeqH2'. apply bool_true_spec in H2. subst. contradiction. inversion H. trivial.
+    + simpl in *. unfold inv. inversion H. apply IHe in H1. clear IHe. subst.
+        destruct H1. 
+        - right. unfold not. intros. intuition.
+        - left. right. split...
+    + inversion H.
+    + inversion H.
+    + inversion H.
+  Qed.
+         
+
+  Lemma BA_Excl_Mid : 
+    forall (e : exp), 
+      pred e -> (Par e (Neg e)) === Id.
+  Proof with auto.
+    intros.
+    split.
+    + intros. simpl in *.
+      unfold union in H0.
+      unfold inv in H0. unfold id.
+      destruct H0. Focus 2. destruct H0. destruct H0. contradiction.
+      destruct H0... apply bool_spec_new in H0...
+    + intros. assert (x = y). apply bool_true_spec in H0...
+      subst. simpl. unfold union. simpl in H0. unfold id in H0. unfold inv.
+      apply (either_or y) in H. intuition.
+  Qed.
+
+  Lemma BA_Contra :
+    forall (e : exp),
+      pred e ->
+      (Seq e (Neg e)) === Drop.
+  Proof with auto.
+    intros. split. 
+    + intros. simpl in *. unfold join in H0.
+      destruct H0.  destruct H0. remember H0 as H0'.
+      clear HeqH0'. apply bool_true_spec in H0. subst. unfold inv in H1.
+      destruct H1. destruct H0. contradiction. destruct H0. subst. contradiction.
+      trivial.
+    + intros. simpl in *. unfold empty in H0. contradiction.
+  Qed.        
+
+
+
 
