Relation.v
@@ -1,0 +1,62 @@
+Set Implicit Arguments.
+
+Require Import Coq.Classes.Equivalence.
+Require Import Coq.Arith.EqNat.
+Require Import Coq.Logic.FunctionalExtensionality.
+Require Import Coq.Setoids.Setoid.
+
+Section Defs.
+
+    Variable A : Type.
+    
+    Definition relation := A -> A -> Prop.
+    
+    Definition union (R1 R2 : relation) : relation :=
+      fun (x y : A) => R1 x y \/ R2 x y.
+    
+    Definition join (R1 R2 : relation) : relation :=
+      fun (x y : A) => exists (z : A), R1 x z /\ R2 z y.
+    
+    Definition empty : relation :=
+      fun (x y : A) => False.
+    
+    Definition id : relation :=
+      fun (x y : A) => x = y.
+    
+    Fixpoint expt (R : relation) (n : nat) : relation :=
+      match n with
+        | 0 => id
+        | S m => join R (expt R m)
+      end.
+    
+    Definition star (R : relation) : relation :=
+      fun (x y : A) => exists n, (expt R n) x y.
+
+    Definition equiv (R1 R2 : relation) :=
+      forall (x y : A), R1 x y <-> R2 x y.
+
+   Definition inv (R : relation) : relation :=
+     fun (x y : A) => ((R x y) /\ False) \/ (~(R x y) /\ (x = y)).
+  
+  Definition contains (R1 R2 : relation) : Prop :=
+     forall (x y : A), R1 x y -> R2 x y.
+
+  End Defs.
+
+  Instance Equivalence_equiv `(A : Type) : Equivalence (@equiv A).
+  Proof with auto.
+    split; unfold equiv.
+    + unfold Reflexive.
+      intros. intuition.
+    + unfold Symmetric.
+      intros. symmetry. apply H.
+    + unfold Transitive.
+      intros.
+      split... 
+      - intros.
+        apply H0.
+        apply H...
+      - intros.
+        apply H.
+        apply H0...
+  Qed.
