Makefile
@@ -1,0 +1,19 @@
+MODULES := \
+  Relation \
+  Syntax \
+  Semantics \
+  BooleanAlgebraAxioms \
+
+VS := $(MODULES:%=%.v)
+
+.PHONY: all clean
+
+all : Makefile.coq
+	$(MAKE) -f Makefile.coq
+
+Makefile.coq: Makefile $(VS)
+	coq_makefile $(VS) -o Makefile.coq
+
+clean: Makefile.coq
+	$(MAKE) -f Makefile.coq clean
+	rm -f Makefile.coq
